module plfa.Induction where
import Relation.Binary.PropositionalEquality as Eq
open Eq using (_≡_; refl; cong; sym)
open Eq.≡-Reasoning using (begin_; _≡⟨⟩_; _≡⟨_⟩_; _∎)
open import Data.Nat using (ℕ; zero; suc; _+_; _*_; _∸_)

+-assoc : ∀ (m n p : ℕ) → (m + n) + p ≡ m + (n + p)
+-assoc zero n p =
  begin
    (zero + n) + p
  ≡⟨⟩
    n + p
  ≡⟨⟩
    zero + (n + p)
  ∎
+-assoc (suc m) n p =
  begin
    (suc m + n) + p
  ≡⟨⟩
    suc (m + n) + p
  ≡⟨⟩
    suc ((m + n) + p)
  ≡⟨ cong suc (+-assoc m n p) ⟩
    suc (m +(n + p))
  ≡⟨⟩
    suc m + (n + p)
  ∎

+-identityʳ : ∀ (m : ℕ) → m + zero ≡ m
+-identityʳ zero =
  begin
    zero + zero
  ≡⟨⟩
    zero
  ∎
+-identityʳ (suc m) =
  begin
    suc m + zero
  ≡⟨⟩
    suc (m + zero)
  ≡⟨ cong suc (+-identityʳ m) ⟩
    suc m
  ∎

+-suc : ∀ (m n : ℕ) → m + suc n ≡ suc (m + n)
+-suc zero n =
  begin
    zero + suc n
  ≡⟨⟩
    suc n
  ≡⟨⟩
    suc (zero + n)
  ∎
+-suc (suc m) n =
  begin
    suc m + suc n
  ≡⟨⟩
    suc (m + suc n)
  ≡⟨ cong suc (+-suc m n) ⟩
    suc (suc (m + n))
  ∎

+-comm : ∀ (m n : ℕ) → m + n ≡ n + m
+-comm m zero =
  begin
    m + zero
  ≡⟨ +-identityʳ m ⟩
    m
  ≡⟨⟩
    zero + m
  ∎
+-comm m (suc n) =
  begin
    m + (suc n)
  ≡⟨ +-suc m n ⟩
    suc (m + n)
  ≡⟨ cong suc (+-comm m n) ⟩
    suc (n + m)
  ≡⟨⟩
    suc n + m
  ∎


+-assoc' : ∀ (m n p : ℕ) → (m + n) + p ≡ m + (n + p)
+-assoc' zero n p = refl
+-assoc' (suc m) n p rewrite +-assoc' m n p = refl

+-identity' : ∀ (n : ℕ) → n + zero ≡ n
+-identity' zero = refl
+-identity' (suc n) rewrite +-identity' n = refl

+-suc' : ∀ (m n : ℕ) → m + suc n ≡ suc (m + n)
+-suc' zero n = refl
+-suc' (suc m) n rewrite +-suc' m n = refl

+-comm' : ∀ (m n : ℕ) → m + n ≡ n + m
+-comm' m zero rewrite +-identity' m = refl
+-comm' m (suc n) rewrite +-suc' m n | +-comm' m n = refl

+-swap : ∀ (m n p : ℕ) → m + (n + p) ≡ n + (m + p)
+-swap m n p =
  begin
    m + (n + p)
  ≡⟨  sym (+-assoc m n p)  ⟩
    (m + n) + p
  ≡⟨ {!(+-comm m n)!} ⟩
    (n + m) + p
  ≡⟨ +-assoc n m p ⟩
    n + (m + p)
  ∎

*-distrib-+ : ∀ (m n p : ℕ) → (m + n) * p ≡ m * p + n * p
*-distrib-+ m n zero =
  begin {!!}
*-distrib-+ m n (suc p) = {!!} 
